update

lib/test.hs
@@ -1,0 +1,50 @@
+module Test where
+
+import qualified Prelude
+
+type Empty = () -- empty inductive
+
+data StateMachine =
+   St_start
+ | St_step
+ | St_end
+
+type Protocols2 =
+  StateMachine
+  -- singleton inductive, whose constructor was Pt_state_machine2
+  
+data TNetwork_type =
+   Build_TNetwork_type
+
+data TNetwork_type2 =
+   TNetwork_type2a2
+ | TNetwork_type2b2
+
+data TNetwork_type3 =
+   TNetwork_type2a
+ | TNetwork_type2b
+
+data TAuth_type =
+   Build_TAuth_type
+
+data TConnection_type =
+   Build_TConnection_type
+
+data TConnection_type2 =
+   Build_TConnection_type2
+
+data Diagonalization =
+   Network TNetwork_type
+ | Network2 TNetwork_type2
+ | Network3 TNetwork_type3
+ | Auth TAuth_type
+ | Connection TConnection_type
+ | Connection2 TConnection_type2
+ | Empty0 Empty
+ | Unit
+ | Bool
+ | CoProd
+ | StateMachine1 StateMachine
+ | Protocols22 Protocols2
+ | String
+
