lib/test.ml
@@ -1,0 +1,46 @@
+
+type empty = |
+
+type stateMachine =
+| St_start
+| St_step
+| St_end
+
+type protocols2 =
+  stateMachine
+  (* singleton inductive, whose constructor was Pt_state_machine2 *)
+
+type tNetwork_type =
+| Build_TNetwork_type
+
+type tNetwork_type2 =
+| TNetwork_type2a2
+| TNetwork_type2b2
+
+type tNetwork_type3 =
+| TNetwork_type2a
+| TNetwork_type2b
+
+type tAuth_type =
+| Build_TAuth_type
+
+type tConnection_type =
+| Build_TConnection_type
+
+type tConnection_type2 =
+| Build_TConnection_type2
+
+type diagonalization =
+| Network of tNetwork_type
+| Network2 of tNetwork_type2
+| Network3 of tNetwork_type3
+| Auth of tAuth_type
+| Connection of tConnection_type
+| Connection2 of tConnection_type2
+| Empty of empty
+| Unit
+| Bool
+| CoProd
+| StateMachine1 of stateMachine
+| Protocols22 of protocols2
+| String
